

Zadanie 1

Wyznaczyć rząd macierzy

a) $A = \begin{bmatrix} 1 & 2 \\ 3 & 6 \end{bmatrix}$

b) $B = \begin{bmatrix} 1 & 0 \\ 0 & 1 \end{bmatrix}$

c) $C = \begin{bmatrix} 1 & 2 & 3 \\ 4 & 5 & 6 \end{bmatrix}$

d) $D = \begin{bmatrix} 1 & 2 & 3 \\ 2 & 4 & 6 \\ 3 & 6 & 9 \end{bmatrix}$

e) $E = \begin{bmatrix} 0 & 1 & 2 \\ 0 & 0 & 0 \\ 0 & 0 & 1 \end{bmatrix}$

f) $F = \begin{bmatrix} 1 & 2 & 3 & 4 \\ 0 & 1 & 2 & 3 \\ 0 & 0 & 1 & 2 \end{bmatrix}$

g) $G = \begin{bmatrix} 2 & 4 & 1 \\ 0 & 0 & 0 \\ 1 & 2 & 0 \end{bmatrix}$

h) $H = \begin{bmatrix} 1 & 2 & 3 & 4 \\ 2 & 4 & 6 & 8 \\ 0 & 0 & 0 & 0 \\ 1 & 0 & 1 & 0 \end{bmatrix}$

Zadanie 2

Wyznaczyć macierz odwrotną do podanej macierzy:

a) $A = \begin{bmatrix} 2 & 3 \\ 1 & 4 \end{bmatrix}$

b) $B = \begin{bmatrix} 5 & -2 \\ 7 & 1 \end{bmatrix}$

c) $C = \begin{bmatrix} 0 & 1 \\ -1 & 2 \end{bmatrix}$

d) $D = \begin{bmatrix} 1 & 2 & 3 \\ 0 & 1 & 4 \\ 5 & 6 & 0 \end{bmatrix}$

e) $E = \begin{bmatrix} 3 & 0 & 2 \\ 2 & 0 & -2 \\ 0 & 1 & 1 \end{bmatrix}$

$$\text{f) } F = \begin{bmatrix} 4 & 7 & 2 \\ 3 & 6 & 1 \\ 2 & 5 & 3 \end{bmatrix}$$

$$\text{g) } G = \begin{bmatrix} 1 & 0 & 2 & -1 \\ 3 & 0 & 0 & 5 \\ 2 & 1 & 4 & -3 \\ 1 & 0 & 5 & 0 \end{bmatrix}$$

$$\text{h) } H = \begin{bmatrix} 2 & 0 & 1 & 3 \\ 1 & 1 & 0 & 0 \\ 0 & 2 & 1 & 1 \\ 4 & 0 & 1 & 2 \end{bmatrix}$$

Zadanie 3

Rozwiązać równania macierzowe

$$\text{a) } AX = B, \quad \text{gdzie } A = \begin{bmatrix} 2 & 1 \\ 3 & 4 \end{bmatrix}, \quad B = \begin{bmatrix} 1 \\ 2 \end{bmatrix}$$

$$\text{b) } XA = B, \quad \text{gdzie } A = \begin{bmatrix} 1 & 0 \\ -2 & 3 \end{bmatrix}, \quad B = \begin{bmatrix} 4 & 1 \\ 2 & 0 \end{bmatrix}$$

$$\text{c) } AX = C, \quad \text{gdzie } A = \begin{bmatrix} 1 & 2 & 3 \\ 0 & 1 & 4 \\ 5 & 6 & 0 \end{bmatrix}, \quad C = \begin{bmatrix} 1 \\ 0 \\ -1 \end{bmatrix}$$

$$\text{d) } AX + B = C, \quad \text{gdzie}$$

$$A = \begin{bmatrix} 1 & 2 \\ 3 & 4 \end{bmatrix}, \quad B = \begin{bmatrix} 1 \\ -1 \end{bmatrix}, \quad C = \begin{bmatrix} 6 \\ 9 \end{bmatrix}$$

$$\text{e) } XA - B = C, \quad \text{gdzie}$$

$$A = \begin{bmatrix} 2 & 0 \\ 1 & 3 \end{bmatrix}, \quad B = \begin{bmatrix} 1 & 1 \\ 0 & 2 \end{bmatrix}, \quad C = \begin{bmatrix} 3 & 1 \\ 2 & 4 \end{bmatrix}$$

$$\text{f) } AX - BX = C, \quad \text{gdzie}$$

$$A = \begin{bmatrix} 4 & 1 \\ 0 & 2 \end{bmatrix}, \quad B = \begin{bmatrix} 1 & 1 \\ 0 & 1 \end{bmatrix}, \quad C = \begin{bmatrix} 3 & 0 \\ 0 & 1 \end{bmatrix}$$

$$\text{g) }$$

$$AX + C = BX - D$$

gdzie:

$$A = \begin{bmatrix} 2 & 1 \\ 0 & 3 \end{bmatrix}, \quad B = \begin{bmatrix} 1 & 4 \\ 2 & 1 \end{bmatrix}, \quad C = \begin{bmatrix} 5 & 2 \\ 1 & -1 \end{bmatrix}, \quad D = \begin{bmatrix} 3 & 0 \\ 2 & 4 \end{bmatrix}$$